pulse/examples/dsls/mini_steel/Pulse.Soundness.Par.fst
@@ -1,0 +1,30 @@
+module Pulse.Soundness.Par
+
+open FStar.Reflection
+open Refl.Typing
+open Pulse.Elaborate.Pure
+open Pulse.Soundness.Common
+open Pulse.Elaborate.Core
+
+module PT = Pulse.Typing
+
+module RT = Refl.Typing
+
+let par_soundness
+  (#f:stt_env)
+  (#g:PT.env)
+  (#u:universe)
+  (#aL #aR:term)
+  (#preL #postL:term)
+  (#preR #postR:term)
+  (#eL #eR:term)
+  (aL_typing:RT.typing (PT.extend_env_l f g) aL (pack_ln (Tv_Type u)))
+  (aR_typing:RT.typing (PT.extend_env_l f g) aR (pack_ln (Tv_Type u)))
+  (preL_typing:RT.typing (PT.extend_env_l f g) preL vprop_tm)
+  (postL_typing:RT.typing (PT.extend_env_l f g) postL (mk_arrow (aL, Q_Explicit) vprop_tm))
+  (preR_typing:RT.typing (PT.extend_env_l f g) preR vprop_tm)
+  (postR_typing:RT.typing (PT.extend_env_l f g) postR (mk_arrow (aR, Q_Explicit) vprop_tm))
+  (eL_typing:RT.typing (PT.extend_env_l f g) eL (mk_stt_comp u aL preL postL))
+  (eR_typing:RT.typing (PT.extend_env_l f g) eR (mk_stt_comp u aR preR postR))
+
+  = admit ()
