pulse/examples/dsls/mini_steel/Pulse.Soundness.Par.fsti
@@ -1,0 +1,38 @@
+module Pulse.Soundness.Par
+
+open FStar.Reflection
+open Refl.Typing
+open Pulse.Elaborate.Pure
+open Pulse.Elaborate.Core
+
+module RT = Refl.Typing
+
+let par_post (u:universe) (aL aR:term) (postL postR:term) (x:var) : term =
+  let x_tm = var_as_term x in
+  let postL = pack_ln (Tv_App postL (mk_fst u u aL aR x_tm, Q_Explicit)) in
+  let postR = pack_ln (Tv_App postR (mk_snd u u aL aR x_tm, Q_Explicit)) in
+  let post = mk_star postL postR in
+  RT.open_or_close_term' post (RT.CloseVar x) 0
+
+val par_soundness
+  (#g:env)
+  (#u:universe)
+  (#aL #aR:term)
+  (#preL #postL:term)
+  (#preR #postR:term)
+  (#eL #eR:term)
+  (x:var{None? (RT.lookup_bvar g x)})
+  (aL_typing:RT.typing g aL (pack_ln (Tv_Type u)))
+  (aR_typing:RT.typing g aR (pack_ln (Tv_Type u)))
+  (preL_typing:RT.typing g preL vprop_tm)
+  (postL_typing:RT.typing g postL (mk_arrow (aL, Q_Explicit) vprop_tm))
+  (preR_typing:RT.typing g preR vprop_tm)
+  (postR_typing:RT.typing g postR (mk_arrow (aR, Q_Explicit) vprop_tm))
+  (eL_typing:RT.typing g eL (mk_stt_comp u aL preL postL))
+  (eR_typing:RT.typing g eR (mk_stt_comp u aR preR postR))
+
+  : GTot (RT.typing g
+                    (mk_par u aL aR preL postL preR postR eL eR)
+                    (mk_stt_comp u (mk_tuple2 u u aL aR)
+                       (mk_star preL preR)
+                       (mk_abs (mk_tuple2 u u aL aR) Q_Explicit (par_post u aL aR postL postR x))))
